---
anki_linked: 0
raisonnements:
outils:
kh_n:
display_title: produit_exponentielle_complexe
---
# Untitled

> [!objectif]
>$$
> \forall(t,t') \in \mathbb{R}^2,e^{it}\times e^{it'}=e^{i(t+t')}
>  $$
### Démonstration

Soit $(t,t') \in \mathbb{R}^2$
$e^{it}\times e^{it'}=(\cos(t)+i\sin(t))(\cos(t')+i\sin(t'))$
Donc $e^{it}\times e^{it'}=\cos(t)\cos(t')-\sin(t)\sin(t')+i(\sin(t')\cos(t)+\sin(t)\cos(t'))$
Donc $e^{it}\times e^{it'}=\cos(t+t')+i\sin(t+t')=e^{i(t+t')}$

D'où le résultat $e^{it}\times e^{it'}=e^{i(t+t')}$
#### Remarques


